examples/Sek/SWSek_proof.v
@@ -127,6 +127,25 @@ End ForallConseqLemmas.
 
 
 
+
+(* Hint Extern 1 (RegisterSpec swchunk_create) =>
+	match goal with R: Whtype _ _ |- _ => Provide (@swchunk_create_spec_of _ _ _ _ R) end. *)
+
+	Ltac xspec_registered f ::=
+		ltac_database_get database_spec f;
+		try match goal with |- ?S -> _ =>
+			match S with context[Whtype _ _] =>
+				match goal with R: Whtype _ _ |- _ =>
+					let H := fresh in
+					intros H;
+					specializes H R;
+					revert H
+				end
+			end
+		end.
+
+
+
 (* ******************************************************* *)
 (** ** Representation predicates *)
 
@@ -189,6 +208,10 @@ Lemma SekExtend_trans : forall A (IA: Inhab A) (M2 M1 M3: SekMem A),
 	SekExtend M1 M3.
 Admitted.
 
+Lemma SekExtend_empty : forall A (IA: Inhab A) (M: SekMem A),
+	SekExtend SM_Empty M.
+Proof using. unfolds~ SekExtend. Qed.
+
 Hint Resolve SekExtend_trans.
 
 #[global]
@@ -202,7 +225,16 @@ Definition SWSek_vconcat A (v: view_) (Lf Lb: listW A) (LLm: listW (listW A)) : 
 
 Lemma SWSek_vconcat_eq : forall A (v: view_) (Lf Lb: listW A) (LLm: listW (listW A)),
 	SWSek_vconcat v Lf Lb LLm = vapp v Lf (vapp v (concat (list_of_listW LLm)) Lb).
-Proof. auto. Qed.
+Proof using. auto. Qed.
+
+Lemma SWSek_neq_vconcat : forall A (v1 v2: view_) (Lf Lb: listW A) (LLm: listW (listW A)),
+	v1 <> v2 ->
+	SWSek_vconcat v2 Lb Lf LLm = SWSek_vconcat v1 Lf Lb LLm.
+Proof using. intros. destruct v1; destruct v2; simpl; rew_list~; false. Qed. 
+
+Lemma SWSek_vconcat_vcons_l : forall A (v: view_) (Lf Lb: listW A) (LLm: listW (listW A)) (X: weighted_ A),
+	SWSek_vconcat v (vcons v X Lf) Lb LLm = vcons v X (SWSek_vconcat v Lf Lb LLm).
+Proof using. intros. unfold SWSek_vconcat. rew_list~. Qed.
 
 Lemma SWSek_vconcat_absorb_left : forall A (v: view_) (Lf Lb: listW A) (LLm: listW (listW A)),
 	SWSek_vconcat v Lf Lb LLm = SWSek_vconcat v nil Lb (vcons v (Wlist_of_listW Lf) LLm).
@@ -212,6 +244,10 @@ Admitted.
 Definition SWSek_middle_full A (LLm: listW (listW A)) : Prop :=
 	ForallConseq (fun c1 c2 => length c1 + length c2 > K) (list_of_listW LLm).
 
+
+Lemma SWSek_middle_full_empty : forall A,
+	(SWSek_middle_full (A := A)) nil.
+Proof using. intros. unfold SWSek_middle_full. apply ForallConseq_nil. Qed.
 
 Lemma SWSek_middle_full_vcons_full : forall A (v: view_) (L: listW A) (LLm: listW (listW A)),
 	IsFull L ->
@@ -250,6 +286,12 @@ Fixpoint depth a (s: swsek_ a) : int :=
 	|	SWSek_Level _ s' _ => 1 + depth s'
 	end.
 
+Lemma depth_pos : forall a (s: swsek_ a),
+	0 <= depth s.
+Proof using. intros. induction~ s. Qed.
+
+Hint Resolve depth_pos.
+
 Definition SWSekOf_Level (pf pb: bool) (v: view_) a A {IA: Inhab a} {EA: Enc a} (RChunk: RChunkType A a)
 	(L: listW A) (sides: loc) (LLm: listW (listW A)) (w: int) : hprop :=
 	\exists f b Lf Lb,
@@ -267,6 +309,30 @@ Lemma SWSekOf_Level_eq : forall (pf pb: bool) (v: view_) a A (IA: Inhab a) (EA: 
 			b ~> RChunk Lb \*
 			\[SWSek_inv_gen pf pb v L Lf Lb LLm w].
 Proof using. auto. Qed.
+
+Lemma SWSekOf_Level_change_view : forall (pf1 pb1: bool) (v1 v2: view_) a A (IA: Inhab a) (EA: Enc a) (RChunk: RChunkType A a)
+	(L: listW A) (sides: loc) (LLm: listW (listW A)) (w: int),
+	let sl := vxor v1 v2 in
+	let (pf2, pb2) := vexchange sl pf1 pb1 in
+	SWSekOf_Level pf1 pb1 v1 RChunk L sides LLm w ==>
+	SWSekOf_Level pf2 pb2 v2 RChunk L sides LLm w.
+Proof using.
+	intros. subst sl. tests~: (v1 = v2); rew_list~; simpl.
+	{ xsimpl. }
+	{ xchange SWSekOf_Level_eq ;=> f b Lf Lb Hsides I.
+		rewrite SWSekOf_Level_eq. xsimpl.
+		{ rewrites~ (>> neq_vlist2 v1). }
+		{ lets [Iconcat Ifull Iweight Ipf Ipb]: I. constructors~. rewrites~ (>> SWSek_neq_vconcat v1). } }
+Qed.
+
+Lemma SWSekOf_Level_change_view_populated : forall (v1 v2: view_) a A (IA: Inhab a) (EA: Enc a) (RChunk: RChunkType A a)
+	(L: listW A) (sides: loc) (LLm: listW (listW A)) (w: int),
+	SWSekOf_Level true true v1 RChunk L sides LLm w ==>
+	SWSekOf_Level true true v2 RChunk L sides LLm w.
+Proof using.
+	intros. forwards*: (>> (SWSekOf_Level_change_view true true v1 v2 (a := a) (A := A)) RChunk L sides LLm w).
+	rew_list in H. xchange H.
+Qed.
 
 Definition SWSekOf_IsEmpty a (s: swsek_ a) : Prop :=
 	exists d, s = SWSek_Empty d.
@@ -318,6 +384,12 @@ Lemma SWSekOf_eq_empty : forall a A (IA: Inhab a) (EA: Enc a) (R: Whtype A a)
 		\[L = nil].
 Proof using. auto. Qed.
 
+Lemma SWSekOf_mid_eq_empty : forall a A (IA: Inhab a) (EA: Enc a) (RChunk: RChunkType A a)
+	(M': SekMem (partial_swchunk_ a)) (oo: option owner_) (LLm: listW (listW A)) (d: partial_swchunk_ a),
+	SWSek_Empty d ~> SWSekOf_mid RChunk M' oo LLm =
+		\[LLm = nil].
+Proof using. auto. Qed.
+
 Lemma SWSekOf_eq_level : forall a A (IA: Inhab a) (EA: Enc a) (R: Whtype A a)
 	(M: SekMem a) (oo: option owner_) (L: listW A) (sides: array a) (m: swsek_ (partial_swchunk_ a)) (w: int),
 	SWSek_Level sides m w ~> SWSekOf R M oo L =
@@ -367,29 +439,7 @@ Admitted.
 
 Hint Extern 1 (RegisterSpec mk_swsek_weight_invariant) => Provide mk_swsek_weight_invariant_spec_of.
 
-Lemma read_1 : forall A (IA: Inhab A) (f b: A),
-	[f; b][1] = b.
-Proof. intros. rew_array. case_if. case_if~. math. Qed.
 
-Hint Rewrite read_1 : rew_list.
-
-
-
-(* Hint Extern 1 (RegisterSpec swchunk_create) =>
-	match goal with R: Whtype _ _ |- _ => Provide (@swchunk_create_spec_of _ _ _ _ R) end. *)
-
-Ltac xspec_registered f ::=
-	ltac_database_get database_spec f;
-	try match goal with |- ?S -> _ =>
-		match S with context[Whtype _ _] =>
-			match goal with R: Whtype _ _ |- _ =>
-				let H := fresh in
-				intros H;
-				specializes H R;
-				revert H
-			end
-		end
-	end.
 
 Definition one_if (P: Prop) : int :=
 	If P then 1 else 0.
@@ -397,20 +447,64 @@ Definition one_if (P: Prop) : int :=
 (* Ltac xsimpl_use_credits tt ::=
 	constr:(false). *)
 
+(* Lemma empty_spec_local : forall (empty: val) a A (IA: Inhab a) (EA: Enc a) (R: Whtype A a)
+	(SWCM: SWChunkMem a) (d: a) (oo: option owner_),
+	(Body empty x0__ := Pay (App swchunk_create d oo)) ->
+		SPEC (empty tt)
+			MONO SWCM
+			PRE \[]
+			POST (fun SWCM' c => SWChunkOf_MaybeOwned R SWCM' oo nil). *)
+
 Lemma swsek_push_spec_of : forall a A (IA: Inhab a) (EA: Enc a) (R: Whtype A a)
 	(M: SekMem a) (v: view_) (oo: option owner_) (L: listW A) (s: swsek_ a) (X: weighted_ A) (x: weighted_ a),
-	v = Front ->
 	SPEC (swsek_push v oo s x)
 		MONO M
 		PRE (s ~> SWSekOf R M oo L \* x ~> R X)
 		POST (fun M' s' => s' ~> SWSekOf R M' oo (vcons v X L)).
 Proof using.
-	introv ->.
+	intros.
 	sets_eq n: (depth s). gen a A IA EA R M L X x s. induction_wf IH: (downto 0) n; hide IH.
 	introv Eqn. xcf. xpay_skip. xmatch.
-	{ xlet. xapp. skip. (* base case, not so interesting *) }
-	{ xchanges SWSekOf_eq_level ;=> LLm SWCM M' -> Cl. xchange SWSekOf_Level_eq ;=> f b Lf Lb Hsides Ig.
-		xapp*. xmatch. rew_list. xapp.
+	{ xlet (fun (empty: val) => forall (SWCM: SWChunkMem a),
+			SPEC (empty tt)
+				MONO SWCM
+				PRE \[]
+				POST (fun SWCM' c => c ~> SWChunkOf_MaybeOwned R SWCM' oo nil)).
+		{ xpay_skip. xapp ;=> c SWCM' HE. xsimpl~. }
+
+		xlet (fun pe =>
+		\exists SWCM1 M1',
+		let M1 := SM_Level SWCM1 M1' in
+		\[SekExtend M M1] \*
+		pe ~> PartialSWChunkOf_MaybeOwned R SWCM1 oo nil \*
+		SWSek_Empty d ~> SWSekOf R M oo L \*
+		SekMemory M1 \*
+		x ~> R X).
+		{ xchange SekMemory_eq. destruct M as [| SWCM M'].
+			{ xchange SChunkMemory_empty (weighted_ a). xapp ;=> c SWCM1 HE.
+				xsimpl~ (SM_Empty (A := partial_swchunk_ a)).
+				{ apply SekExtend_empty. (* Lemma extend_empty *) }
+				{ simpl. xsimpl. (* ??? *) } }
+			{ xapp ;=> c SWCM1 HE. xsimpl~ M'. rewrite SekExtend_eq_level. split~. apply SekExtend_refl. } }
+	  xpull ;=> SWCM1 M1'. xpull ;=> HE.
+		xchange SekMemory_eq_level. xapp ;=> b SWCM2 HE1. xapp ;=> f SWCM3 HE2.
+		xmatch. xapp ;=> f1 SWCM4 HE3. simpl in *.
+		(* Monotonie *)
+		xchange~ SWChunkOf_MaybeOwned_Mono SWCM2 SWCM4.
+		xchange~ PartialSWChunkOf_MaybeOwned_Mono SWCM1 SWCM4.
+		sets_eq RChunk: (SWChunkOf_MaybeOwned R SWCM4 oo).
+		xchange* <- (>> SWSekOf_mid_eq_empty RChunk M1' oo partial_empty).
+		subst RChunk.
+		xchange <- SekMemory_eq_level. xapp.
+		{ apply SWSek_middle_full_empty. }
+		{ intros s' M2 HE'. xchange SWSekOf_eq_empty ;=> HL. xsimpl~.
+			{ do 2 applys~ SekExtend_trans. rewrite SekExtend_eq_level. split~. apply SekExtend_refl. }
+			{ rewrite SWSek_vconcat_eq. rew_listx*. }
+			{ skip. (* haffine *) } } }
+	{ xchanges SWSekOf_eq_level ;=> LLm SWCM M' -> Cl.
+		xchange SWSekOf_Level_change_view_populated Front v.
+		xchange SWSekOf_Level_eq ;=> f b Lf Lb Hsides Ig.
+		xapp*. rew_list. xmatch. xapp.
 		xlet (fun '(f1, mid1) =>
 			\exists SWCM1 M1' Lf1 LLm1,
 			let M := SM_Level SWCM M' in
@@ -422,7 +516,7 @@ Proof using.
 			b ~> RChunk Lb \*
 			\[~ IsFull Lf1] \*
 			\[SWSek_middle_full LLm1] \*
-			\[L = SWSek_vconcat Front Lf1 Lb LLm1] \*
+			\[L = SWSek_vconcat v Lf1 Lb LLm1] \*
 			mid1 ~> SWSekOf_mid RChunk M1' oo LLm1 \*
 			SekMemory M1 \*
 			x ~> R X).
@@ -432,13 +526,11 @@ Proof using.
 				(* pourquoi ça marche pas tout de suite? *)
 				do 2 xchange~ SWChunkOf_MaybeOwned_Mono. xchange~ SWSekOf_mid_Mono.
 				xchange RChunk_lift f. xchange* SWSekOf_mid_eq. sets_eq n': (depth mid). xapp~; simpl.
-				{ split.
-					{ skip. } (* lemmas: depth >= 0*)
-					{ subst n n'. math. } }
-				{ intros mid' M1' HE1. xval. xsimpl~ (Wlist_of_listW Lf :: LLm).
+				{ split*. }
+				{ intros mid' M1' HE1. xval. xsimpl~ (vcons v (Wlist_of_listW Lf) LLm).
 					{ apply capacity_spec. }
-					{ applys~ SWSek_middle_full_vcons_full Front. }
-					{ subst L. rewrite* SWSek_vconcat_absorb_left. }
+					{ applys~ SWSek_middle_full_vcons_full v. }
+					{ rewrite~ <- SWSek_vconcat_absorb_left. }
 					{ xchanges <- SWSekOf_mid_eq. fequals. unfold Wlist_of_listW. fequals. applys~ swcinv_sum. } } }
 			{ xvals~. split*.
 				{ apply SChunkExtend_refl. }
@@ -448,6 +540,6 @@ Proof using.
 	xchange <- SekMemory_eq_level. xchange~ SWChunkOf_MaybeOwned_Mono. xchange~ SWSekOf_mid_Mono.
 	xapp~; simpl ;=> s' M2 HE2. xsimpl.
 	{ destruct HE as [HE HES]. destruct~ M2 as [| SWCM2 M2']. destruct HE2 as [HE2 HES2]. split~. }
-	{ rew_list. fequals~. }
-	{ skip. (* credits... *) } }
+	{ rewrites SWSek_vconcat_vcons_l. fequals~. }
+	{ skip. (* credits *) } }
 Qed.
